A12Kernel.lean
@@ -164,6 +164,7 @@ import A12Kernel.Elaboration.DateFragmentFirstFilledComputation
 import A12Kernel.Elaboration.DateRangeFirstFilledComputation
 import A12Kernel.Elaboration.AddressedDateRangeFirstFilledComputation
 import A12Kernel.Elaboration.DateTimeFirstFilledComputation
+import A12Kernel.Elaboration.AddressedDateTimeFirstFilledComputation
 import A12Kernel.Elaboration.FullDateFirstFilledComputation
 import A12Kernel.Elaboration.TimeFirstFilledComputation
 import A12Kernel.Elaboration.StarGroup
